try fixed-window method from lib.exponentiation in ed25519

code/ed25519/Hacl.Impl.Ed25519.Ladder.fst
@@ -13,7 +13,81 @@ module S = Hacl.Spec.Ed25519.Field56.Definition
 module F56 = Hacl.Impl.Ed25519.Field56
 module F51 = Hacl.Impl.Ed25519.Field51
 
-#set-options "--z3rlimit 20 --max_fuel 0 --max_ifuel 0"
+module LE = Lib.Exponentiation
+module BE = Hacl.Impl.Exponentiation
+module BN = Hacl.Bignum
+module SN = Hacl.Spec.Bignum
+module LSeq = Lib.Sequence
+
+#set-options "--z3rlimit 50 --max_fuel 0 --max_ifuel 0"
+
+////////////////////////////////////////////////////
+unfold
+let a_spec = Spec.Ed25519.ext_point
+
+unfold
+let exp : LE.exp a_spec = Spec.Ed25519.mk_ed25519_group
+
+unfold
+let lseq_as_felem (a:LSeq.lseq uint64 5) : GTot Hacl.Spec.Curve25519.Field51.Definition.felem5 =
+  let s0 = LSeq.index a 0 in
+  let s1 = LSeq.index a 1 in
+  let s2 = LSeq.index a 2 in
+  let s3 = LSeq.index a 3 in
+  let s4 = LSeq.index a 4 in
+  (s0, s1, s2, s3, s4)
+
+unfold
+let linv (a:LSeq.lseq uint64 20) : Type0 =
+  Hacl.Spec.Curve25519.Field51.mul_inv_t (lseq_as_felem (LSeq.sub a 0 5)) /\
+  Hacl.Spec.Curve25519.Field51.mul_inv_t (lseq_as_felem (LSeq.sub a 5 5)) /\
+  Hacl.Spec.Curve25519.Field51.mul_inv_t (lseq_as_felem (LSeq.sub a 10 5)) /\
+  Hacl.Spec.Curve25519.Field51.mul_inv_t (lseq_as_felem (LSeq.sub a 15 5))
+
+unfold
+let refl (a:LSeq.lseq uint64 20) : GTot a_spec =
+  let open Hacl.Spec.Curve25519.Field51.Definition in
+  let x = feval (lseq_as_felem (LSeq.sub a 0 5)) in
+  let y = feval (lseq_as_felem (LSeq.sub a 5 5)) in
+  let z = feval (lseq_as_felem (LSeq.sub a 10 5)) in
+  let t = feval (lseq_as_felem (LSeq.sub a 15 5)) in
+  (x, y, z, t)
+
+unfold
+let linv_ctx (a:LSeq.lseq uint64 0) : Type0 = True
+
+
+inline_for_extraction noextract
+let mk_lexp_to_exp : BE.lexp_to_exp U64 20ul 0ul = {
+  BE.a_spec = a_spec;
+  BE.exp = exp;
+  BE.linv_ctx = linv_ctx;
+  BE.linv = linv;
+  BE.refl = refl;
+  }
+
+inline_for_extraction noextract
+val point_add : BE.lmul_st U64 20ul 0ul mk_lexp_to_exp
+let point_add ctx x y xy =
+  Hacl.Impl.Ed25519.PointAdd.point_add xy x y
+
+
+inline_for_extraction noextract
+val point_double : BE.lsqr_st U64 20ul 0ul mk_lexp_to_exp
+let point_double ctx x xx =
+  let h0 = ST.get () in
+  Spec.Ed25519.lemma_fsqr (refl (as_seq h0 x));
+  Hacl.Impl.Ed25519.PointDouble.point_double xx x
+
+
+inline_for_extraction noextract
+let mk_lexp : BE.lexp U64 20ul 0ul = {
+  BE.to = mk_lexp_to_exp;
+  BE.lmul = point_add;
+  BE.lsqr = point_double;
+}
+
+//////////////////////////////////////////////
 
 inline_for_extraction noextract
 val make_point_inf:
@@ -62,113 +136,14 @@ let make_g g =
   (**) assert_norm (Mktuple4?._4 Spec.Ed25519.g ==
     Hacl.Spec.Curve25519.Field51.Definition.as_nat5 (u64 0x00068ab3a5b7dda3, u64 0x00000eea2a5eadbb, u64 0x0002af8df483c27e, u64 0x000332b375274732, u64 0x00067875f0fd78b7) % Spec.Curve25519.prime)
 
-inline_for_extraction noextract
-val ith_bit:
-    k:lbuffer uint8 32ul
-  -> i:size_t{v i < 256} ->
-  Stack uint8
-    (requires fun h -> live h k)
-    (ensures fun h0 z h1 -> h0 == h1 /\ v z <= 1 /\
-        z == Spec.Ed25519.ith_bit (as_seq h0 k) (v i)
-    )
-let ith_bit k i =
-  let q = i >>. 3ul in
-  let r = i &. 7ul in
-  mod_mask_lemma i 3ul;
-  Lib.IntTypes.Compatibility.uintv_extensionality 7ul (mod_mask #U32 3ul);
-  assert (v r == v i % 8);
-  let kq = k.(q) in
-  let z = (kq >>. r) &. u8 1 in
-  mod_mask_lemma (kq >>. r) 1ul;
-  Lib.IntTypes.Compatibility.uintv_extensionality (u8 1) (mod_mask #U8 1ul);
-  z
-
-inline_for_extraction noextract
-val loop_step:
-    b:lbuffer uint64 80ul
-  -> k:lbuffer uint8 32ul
-  -> ctr:size_t{v ctr < 256} ->
-  Stack unit
-    (requires fun h -> live h b /\ live h k /\ disjoint k b /\
-      F51.point_inv_t h (gsub b 0ul 20ul) /\
-      F51.point_inv_t h (gsub b 20ul 20ul)
-    )
-    (ensures  fun h0 _ h1 -> modifies (loc b) h0 h1 /\
-      F51.point_inv_t h1 (gsub b 0ul 20ul) /\
-      F51.point_inv_t h1 (gsub b 20ul 20ul) /\
-
-      (F51.point_eval h1 (gsub b 0ul 20ul), F51.point_eval h1 (gsub b 20ul 20ul)) ==
-      Spec.Ed25519.ladder_step (as_seq h0 k) (v ctr)
-       (F51.point_eval h0 (gsub b 0ul 20ul), F51.point_eval h0 (gsub b 20ul 20ul))
-    )
-
-#push-options "--z3rlimit 60"
-
-let lemma_to_u8_to_u64 (i:uint8) : Lemma (to_u8 (to_u64 i) == i)
-  = ()
-
-let loop_step b k ctr =
-  let nq    = sub b 0ul 20ul in
-  let nqpq  = sub b 20ul 20ul in
-  let nq2   = sub b 40ul 20ul in
-  let nqpq2 = sub b 60ul 20ul in
-  let i  = ith_bit k (255ul -. ctr) in
-  (**) assert (v (255ul -. ctr) == 255 - v ctr);
-  (**) lemma_to_u8_to_u64 i;
-  Hacl.Impl.Ed25519.SwapConditional.swap_conditional_inplace nq nqpq (to_u64 i);
-  Hacl.Impl.Ed25519.PointDouble.point_double nq2 nq;
-  Hacl.Impl.Ed25519.PointAdd.point_add nqpq2 nq nqpq;
-  Hacl.Impl.Ed25519.SwapConditional.swap_conditional nq nqpq nq2 nqpq2 (to_u64 i)
-
-#pop-options
-
-inline_for_extraction noextract
-val point_mul_:
-    b:lbuffer uint64 80ul
-  -> k:lbuffer uint8 32ul ->
-  Stack unit
-    (requires fun h -> live h k /\ live h b /\ disjoint b k /\
-      F51.point_inv_t h (gsub b 0ul 20ul) /\ F51.point_inv_t h (gsub b 20ul 20ul) /\
-      F51.point_eval h (gsub b 0ul 20ul) == Spec.Curve25519.(zero, one, one, zero)
-    )
-    (ensures  fun h0 _ h1 -> modifies (loc b) h0 h1 /\
-       F51.point_inv_t h1 (gsub b 0ul 20ul) /\ F51.point_inv_t h1 (gsub b 20ul 20ul) /\
-       F51.point_eval h1 (gsub b 0ul 20ul) ==
-       Spec.Ed25519.point_mul (as_seq h0 k) (F51.point_eval h0 (gsub b 20ul 20ul))
-    )
-
-#set-options "--z3rlimit 60 --max_fuel 0 --max_ifuel 0"
-
-let point_mul_ b k =
-  let h0 = ST.get() in
-
-  [@inline_let]
-  let spec h0 = Spec.Ed25519.ladder_step (as_seq h0 k) in
-
-  [@inline_let]
-  let acc h : GTot (Spec.Ed25519.ext_point & Spec.Ed25519.ext_point) =
-    F51.point_eval h (gsub b 0ul 20ul), F51.point_eval h (gsub b 20ul 20ul)
-  in
-
-  [@inline_let]
-  let inv h (i:nat{i <= 256}) = modifies (loc b) h0 h /\
-    F51.point_inv_t h (gsub b 0ul 20ul) /\ F51.point_inv_t h (gsub b 20ul 20ul) /\
-    acc h == Lib.LoopCombinators.repeati i (spec h0) (acc h0)
-  in
-
-  Lib.LoopCombinators.eq_repeati0 256 (spec h0) (acc h0);
-  Lib.Loops.for 0ul 256ul inv
-    (fun i ->
-      Lib.LoopCombinators.unfold_repeati 256 (spec h0) (acc h0) (v i);
-      loop_step b k i)
 
 val point_mul:
     result:point
   -> scalar:lbuffer uint8 32ul
   -> q:point ->
   Stack unit
-    (requires fun h -> live h scalar /\ live h q /\ live h result /\
-      F51.point_inv_t h q
+    (requires fun h ->
+      live h scalar /\ live h q /\ live h result /\ F51.point_inv_t h q
     )
     (ensures  fun h0 _ h1 -> modifies (loc result) h0 h1 /\
       F51.point_inv_t h1 result /\
@@ -176,15 +151,18 @@ val point_mul:
     )
 
 let point_mul result scalar q =
+  let h0 = ST.get () in
   push_frame();
-  let b = create 80ul (u64 0) in
-  let nq   = sub b  0ul 20ul in
-  let nqpq = sub b 20ul 20ul in
-  make_point_inf nq;
-  copy nqpq q;
-  point_mul_ b scalar;
-  copy result nq;
+  let a = create 20ul (u64 0) in
+  copy a q;
+  let bscalar = create 4ul (u64 0) in
+  BN.bn_from_bytes_le 32ul scalar bscalar;
+  SN.bn_from_bytes_le_lemma #U64 32 (as_seq h0 scalar);
+
+  make_point_inf result;
+  BE.lexp_fw_raw 20ul 0ul mk_lexp (null uint64) a 4ul 256ul bscalar result 4ul;
   pop_frame()
+
 
 val point_mul_g:
     result:point
